Improve definition of basic semantic judgments

theories/experiments.v
@@ -3,11 +3,88 @@ Require Import Dot.unary_lr.
 Require Import Dot.synLemmas.
 (* Workflow: Use this file for new experiments, and move experiments here in appropriate files once they're done. *)
 
+Implicit Types T: ty.
 Section Sec.
   Context `{HdotG: dotG Σ}.
 
+  Definition uvstp2 Γ T1 T2: iProp Σ :=
+    (□∀ ρ v, ⟦Γ⟧*ρ → |={⊤}=> (⟦T1⟧ ρ v) → ⟦T2⟧ ρ v)%I.
+  Global Arguments uvstp2 /.
+  (* Print uvstp2. *)
+
+  (* To be able to use uvstp2, maybe we can use the following. Since it uses a single WP, it's clear
+   * that we're talking about a single execution of e! That's weaker for non-deterministic
+   * languages, but makes more sense: subtyping is about the same result after all.
+   * However, this also asserts that all expressions are safe???
+   *)
+  Definition istp2 Γ T1 T2 : iProp Σ := (□∀ e ρ, ⟦Γ⟧* ρ →
+                                                 WP e {{v, ⟦T1⟧ ρ v → ⟦T2⟧ ρ v}})%I.
+
+  Lemma dropUpdateFromPremise {A B: iProp Σ}:
+    (□ ((|={⊤}=> A) → |={⊤}=> B) ↔ □ (A → |={⊤}=> B))%I.
+  Proof.
+    iSplit; iIntros "#Himpl !>".
+    - iIntros "HA". by iApply "Himpl".
+    - iIntros ">HA". by iApply "Himpl".
+  Qed.
+
   Context (Γ: list ty).
-  Implicit Types T: ty.
+
+  (* Does the converse direction hold? Do we need it? *)
+  (* Lemma iStpVstp Γ T1 T2: (istp Γ T1 T2 -∗ ivstp Γ T1 T2)%I. *)
+  (* This direction is useful when we have istp as an hypothesis. *)
+  (* What I can easily prove: *)
+
+  Lemma vstpToUvstp T1 T2 : (Γ ⊨v T1 <: T2 → Γ ⊨> T1 <: T2)%I.
+    iIntros "#Hstp !> * #Hg #HT1 !>".
+    by iApply ("Hstp").
+  Qed.
+
+  Lemma iVstpStp T1 T2: (Γ ⊨v T1 <: T2 → Γ ⊨ T1 <: T2)%I.
+  Proof.
+  (*   by iIntros "#Hsub"; iApply istpEqIvstp; iApply vstpToUvstp. *)
+  (* Qed. *)
+    iIntros "#Hsub !> * #Hg HT1".
+    iApply (wp_wand with " [-]"). iApply "HT1". by iIntros; iApply "Hsub".
+  Qed.
+
+  (* Maybe the update is OK; after all, it's part of the definition of weakest
+     preconditions, and it pairs with the later. But it confuses me honestly.
+
+     In any case, once we add pointers typing will clearly depend on resources (such as the heap), so we can just as well deal with it now. *)
+  (* Also, subtyping now implies subtyping after update: *)
+  (* But not viceversa, because |==> P talks about the *existence* of a future resource world
+   where P holds, even though P might be false now. *)
+  Lemma uvstpToVstp T1 T2 : (Γ ⊨> T1 <: T2 → Γ ⊨v T1 <: T2)%I.
+    iIntros "/= #Hstp !> * #Hg #Ht1".
+    Fail iApply "Hstp".
+  Abort.
+
+  Lemma uvstp21 T1 T2: (uvstp2 Γ T1 T2 → uvstp Γ T1 T2)%I.
+  Proof.
+    iIntros "/= #Hstp !> * #Hg".
+    iDestruct ("Hstp" $! ρ v with "Hg") as "H".
+    iIntros "HT1". by iApply "H".
+  Qed.
+
+  (* False. *)
+  Lemma uvstp12 T1 T2: (uvstp Γ T1 T2 -∗ uvstp2 Γ T1 T2)%I.
+  Proof.
+    iIntros "/= #Hstp !> * #Hg".
+    iSpecialize ("Hstp" $! v ρ with "Hg").
+    Fail iMod "Hstp".
+    Fail iApply "Hstp".
+    iIntros "!>".
+  Abort.
+
+  Lemma iStpUvstp2 T1 T2: (istp2 Γ T1 T2 -∗ uvstp2 Γ T1 T2)%I.
+  Proof.
+    iIntros "/= #Hsub !> * #Hg *".
+    iSpecialize ("Hsub" $! (of_val v) with "Hg").
+    rewrite !wp_unfold /wp_pre /=. by iApply "Hsub".
+  Qed.
+
+
 
   (* Locate "|==>". *)
   (* Check @bupd. *)
@@ -24,39 +101,6 @@ Section Sec.
     (|==> ∃ γ, SP γ (uinterp T))%I.
   Proof. by apply saved_pred_alloc. Qed.
 
-  Program Fixpoint wtovdm (dw: dm):
-    (|==> ∃(dv: dm), (True%I: iProp Σ))%I :=
-    (* (|==> )%I := *)
-    match dw with
-      | dtysyn T => _
-      | dvl w =>
-        _
-        (* dvl w (* XXX *) *)
-      | dtysem γ σ =>
-        _
-        (* dtysem γ *)
-    end.
-  Next Obligation.
-    iIntros "** !>".
-    iDestruct (alloc_sp T) as ">Hγ".
-    iDestruct "Hγ" as (γ) "Hsp".
-    by iExists (dtysem _ γ).
-    Grab Existential Variables.
-    constructor.
-  Defined.
-  Next Obligation.
-    iIntros "** !>".
-    by iExists dw.
-  Defined.
-  Next Obligation.
-    iIntros "** !>".
-    by iExists dw.
-  Defined.
-
-  (* Program Definition wtov (w: val): val := *)
-  (*   match w with *)
-  (*     |  *)
-
   Lemma alloc_dtp_tmem_i T ρ:
     ⟦Γ⟧* ρ -∗
     (|==> ∃ γ, defs_interp (TTMem 0 T T) ρ [@ dtysem (idsσ ρ) γ])%I.
@@ -68,103 +112,104 @@ Section Sec.
     rewrite <- idsσ_is_id.
     repeat iSplit; repeat iModIntro; by iIntros "**".
   Qed.
-  (* Print saved_pred_own. *)
-  (* Print Next. *)
-  (* Print savedPredG. *)
-  (* Eval cbn in (∀ A, savedAnythingG Σ (A -c> ▶ ∙)). *)
-  (* Check savedAnythingG. *)
-  (* From iris Require Import algebra.ofe. *)
-  (* Check savedEnvD. *)
-  (* Alternative to savedPredG *)
-  Notation savedEnvDG := (savedAnythingG Σ (listVlC -c> vlC -c> ▶ ∙)%CF).
-  Notation savedEnvDΣ := (savedAnythingΣ (listVlC -c> vlC -c> ▶ ∙)).
 
-  (* (* Notation savedEnvDG := (savedAnythingG Σ (listVlC -c> vlC -c> ▶ ∙)). *) *)
-  (* (* Notation savedEnvDΣ := (savedAnythingΣ (listVlC -c> vlC -c> ▶ ∙)). *) *)
+  (* (* Print saved_pred_own. *) *)
+  (* (* Print Next. *) *)
+  (* (* Print savedPredG. *) *)
+  (* (* Eval cbn in (∀ A, savedAnythingG Σ (A -c> ▶ ∙)). *) *)
+  (* (* Check savedAnythingG. *) *)
+  (* (* From iris Require Import algebra.ofe. *) *)
+  (* (* Check savedEnvD. *) *)
+  (* (* Alternative to savedPredG *) *)
+  (* Notation savedEnvDG := (savedAnythingG Σ (listVlC -c> vlC -c> ▶ ∙)%CF). *)
+  (* Notation savedEnvDΣ := (savedAnythingΣ (listVlC -c> vlC -c> ▶ ∙)). *)
+
+  (* (* (* Notation savedEnvDG := (savedAnythingG Σ (listVlC -c> vlC -c> ▶ ∙)). *) *) *)
+  (* (* (* Notation savedEnvDΣ := (savedAnythingΣ (listVlC -c> vlC -c> ▶ ∙)). *) *) *)
+  (* (* (* Print saved_anything_own. *) *) *)
+  (* (* (* Print savedAnythingG. *) *) *)
+  (* (* (* Print cFunctor. *) *) *)
+  (* (* Print savedPredG. *) *)
+  (* (* Print saved_pred_own. *) *)
+
   (* (* Print saved_anything_own. *) *)
-  (* (* Print savedAnythingG. *) *)
-  (* (* Print cFunctor. *) *)
-  (* Print savedPredG. *)
-  (* Print saved_pred_own. *)
+  (* Context `{savedEnvDG}. *)
+  (* Program Definition saved_envDG_own (γ : gname) (Φ : listVlC -n> vlC -n> iProp Σ): iProp Σ := *)
+  (*   saved_anything_own (F := listVlC -c> vlC -c> ▶ ∙) γ (λ ρ, λne v, Next (Φ ρ v)). *)
 
-  (* Print saved_anything_own. *)
-  Context `{savedEnvDG}.
-  Program Definition saved_envDG_own (γ : gname) (Φ : listVlC -n> vlC -n> iProp Σ): iProp Σ :=
-    saved_anything_own (F := listVlC -c> vlC -c> ▶ ∙) γ (λ ρ, λne v, Next (Φ ρ v)).
+  (* Instance saved_envDG_own_contractive γ: *)
+  (*   Contractive *)
+  (*               (saved_envDG_own γ: (listVlC -n> vlC -n> iProp Σ) → iProp Σ). *)
+  (* Proof. *)
+  (*   solve_proper_core ltac:(fun _ => *)
+  (*                   first [ intros ? ?; progress simpl | by auto | f_contractive | f_equiv ]). *)
 
-  Instance saved_envDG_own_contractive γ:
-    Contractive
-                (saved_envDG_own γ: (listVlC -n> vlC -n> iProp Σ) → iProp Σ).
-  Proof.
-    solve_proper_core ltac:(fun _ =>
-                    first [ intros ? ?; progress simpl | by auto | f_contractive | f_equiv ]).
+  (*   (* solve_proper_prepare. *) *)
 
-    (* solve_proper_prepare. *)
+  (*   (* repeat first [eassumption | first [ intros ? ?; progress simpl | by auto | f_contractive | f_equiv ]]. *) *)
+  (*   (* cbn in H0. *) *)
+  (*   (* solve [apply H0]. *) *)
+  (*   (* Restart. *) *)
+  (*   (* (* Summarizes to: *) *) *)
+  (*   (* solve_proper_core ltac:(fun _ => *) *)
+  (*   (*                 first [ intros ? ?; progress simpl | by auto | f_contractive | f_equiv | apply H0 ]). *) *)
+  (*   (* (* But that is really fragile.*) *) *)
+  (* Qed. *)
 
-    (* repeat first [eassumption | first [ intros ? ?; progress simpl | by auto | f_contractive | f_equiv ]]. *)
-    (* cbn in H0. *)
-    (* solve [apply H0]. *)
-    (* Restart. *)
-    (* (* Summarizes to: *) *)
-    (* solve_proper_core ltac:(fun _ => *)
-    (*                 first [ intros ? ?; progress simpl | by auto | f_contractive | f_equiv | apply H0 ]). *)
-    (* (* But that is really fragile.*) *)
-  Qed.
+  (* Lemma saved_envDG_alloc_strong (G : gset gname) (Φ : listVlC -n> vlC -n> iProp Σ) : *)
+  (*   (|==> ∃ γ, ⌜γ ∉ G⌝ ∧ saved_envDG_own γ Φ)%I. *)
+  (* Proof. iApply saved_anything_alloc_strong. Qed. *)
 
-  Lemma saved_envDG_alloc_strong (G : gset gname) (Φ : listVlC -n> vlC -n> iProp Σ) :
-    (|==> ∃ γ, ⌜γ ∉ G⌝ ∧ saved_envDG_own γ Φ)%I.
-  Proof. iApply saved_anything_alloc_strong. Qed.
+  (* Lemma saved_envDG_alloc (Φ : listVlC -n> vlC -n> iProp Σ) : *)
+  (*   (|==> ∃ γ, saved_envDG_own γ Φ)%I. *)
+  (* Proof. iApply saved_anything_alloc. Qed. *)
 
-  Lemma saved_envDG_alloc (Φ : listVlC -n> vlC -n> iProp Σ) :
-    (|==> ∃ γ, saved_envDG_own γ Φ)%I.
-  Proof. iApply saved_anything_alloc. Qed.
+  (* (* We put the `x` on the outside to make this lemma easier to apply. *) *)
+  (* Lemma saved_envDG_agree1 `{savedPredG Σ A} γ Φ Ψ x : *)
+  (*   saved_envDG_own γ Φ -∗ saved_envDG_own γ Ψ -∗ ▷ (Φ x ≡ Ψ x). *)
+  (*   unfold saved_envDG_own. iIntros "#HΦ #HΨ". *)
+  (*   Import uPred. *)
+  (*   iApply later_equivI. *)
+  (*   (* Check @saved_anything_agree. *) *)
+  (*   (* Eval hnf in (listVlC -c> vlC -c> ▶ iProp Σ)%CF. *) *)
+  (*   iDestruct (saved_anything_agree (F := listVlC -c> vlC -c> ▶ ∙) with "HΦ HΨ") as "Heq". *)
+  (*   simpl. *)
 
-  (* We put the `x` on the outside to make this lemma easier to apply. *)
-  Lemma saved_envDG_agree1 `{savedPredG Σ A} γ Φ Ψ x :
-    saved_envDG_own γ Φ -∗ saved_envDG_own γ Ψ -∗ ▷ (Φ x ≡ Ψ x).
-    unfold saved_envDG_own. iIntros "#HΦ #HΨ".
-    Import uPred.
-    iApply later_equivI.
-    (* Check @saved_anything_agree. *)
-    (* Eval hnf in (listVlC -c> vlC -c> ▶ iProp Σ)%CF. *)
-    iDestruct (saved_anything_agree (F := listVlC -c> vlC -c> ▶ ∙) with "HΦ HΨ") as "Heq".
-    simpl.
+  (*   (* Check @ofe_fun_equivI. *) *)
+  (*   iDestruct (@ofe_fun_equivI _ (listVlC) (λ _, vlC -n> laterC (iProp Σ)) (λ ρ, λne v, Next (Φ ρ v)) (λ ρ, λne v, Next (Ψ ρ v))) as "[Heq1 _]". *)
+  (*   Fail iSpecialize ("Heq1" with "Heq"). *)
+  (*   Abort. *)
+  (* (* (*   by iDestruct ("Heq1" with "Heq") as "?". *) *) *)
 
-    (* Check @ofe_fun_equivI. *)
-    iDestruct (@ofe_fun_equivI _ (listVlC) (λ _, vlC -n> laterC (iProp Σ)) (λ ρ, λne v, Next (Φ ρ v)) (λ ρ, λne v, Next (Ψ ρ v))) as "[Heq1 _]".
-    Fail iSpecialize ("Heq1" with "Heq").
-    Abort.
-  (* (*   by iDestruct ("Heq1" with "Heq") as "?". *) *)
+  (* (* (*   simpl. *) *) *)
+  (* (* (*   Unset Printing Notations. *) *) *)
+  (* (* (*   Set Printing Implicit. *) *) *)
+  (* (* (*   simpl in *. *) *) *)
+  (* (* (*   iDestruct ("Heq1" with "Heq") as "?". *) *) *)
+  (* (* (*   iApply "Heq1". *) *) *)
 
-  (* (*   simpl. *) *)
-  (* (*   Unset Printing Notations. *) *)
-  (* (*   Set Printing Implicit. *) *)
-  (* (*   simpl in *. *) *)
-  (* (*   iDestruct ("Heq1" with "Heq") as "?". *) *)
-  (* (*   iApply "Heq1". *) *)
+  (* (* (*  "Heq" : (λ (ρ : listVlC) (v : vlC), Next (Φ ρ v)) *) *) *)
+  (* (* (*         ≡ (λ (ρ : listVlC) (v : vlC), Next (Ψ ρ v)) *) *) *)
+  (* (* (*   iDestruct (ofe_fun_equivI with "Heq"). as "?". *) *) *)
+  (* (* (*   by iDestruct (ofe_fun_equivI with "Heq") as "?". *) *) *)
+  (* (* (* Qed. *) *) *)
+
+  (* (* Lemma saved_envDG_agree `{savedPredG Σ A} γ Φ Ψ x y : *) *)
+  (* (*   saved_envDG_own γ Φ -∗ saved_envDG_own γ Ψ -∗ ▷ (Φ x y ≡ Ψ x y). *) *)
+  (* (* Proof. *) *)
+  (* (*   unfold saved_envDG_own. iIntros "#HΦ #HΨ /=". *) *)
+  (* (*   Import uPred. *) *)
+  (* (*   iApply later_equivI. *) *)
+  (* (*   Check @saved_anything_agree. *) *)
+  (* (*   Eval hnf in (listVlC -c> vlC -c> ▶ iProp Σ)%CF. *) *)
+  (* (*   iDestruct (saved_anything_agree (F := listVlC -c> vlC -c> ▶ ∙) with "HΦ HΨ") as "Heq". *) *)
+  (* (*   Check @ofe_fun_equivI. *) *)
+  (* (*   epose proof (@ofe_fun_equivI _ (listVlC) (λ _, vlC -n> laterC (iProp Σ)) (λne ρ, λne v, CofeMor Next (Φ ρ v)) (λ ρ, λne v, Next (Ψ ρ v))). *) *)
+  (* (*   iDestruct (H0 with "Heq") as "?". *) *)
 
   (* (*  "Heq" : (λ (ρ : listVlC) (v : vlC), Next (Φ ρ v)) *) *)
   (* (*         ≡ (λ (ρ : listVlC) (v : vlC), Next (Ψ ρ v)) *) *)
   (* (*   iDestruct (ofe_fun_equivI with "Heq"). as "?". *) *)
   (* (*   by iDestruct (ofe_fun_equivI with "Heq") as "?". *) *)
   (* (* Qed. *) *)
-
-  (* Lemma saved_envDG_agree `{savedPredG Σ A} γ Φ Ψ x y : *)
-  (*   saved_envDG_own γ Φ -∗ saved_envDG_own γ Ψ -∗ ▷ (Φ x y ≡ Ψ x y). *)
-  (* Proof. *)
-  (*   unfold saved_envDG_own. iIntros "#HΦ #HΨ /=". *)
-  (*   Import uPred. *)
-  (*   iApply later_equivI. *)
-  (*   Check @saved_anything_agree. *)
-  (*   Eval hnf in (listVlC -c> vlC -c> ▶ iProp Σ)%CF. *)
-  (*   iDestruct (saved_anything_agree (F := listVlC -c> vlC -c> ▶ ∙) with "HΦ HΨ") as "Heq". *)
-  (*   Check @ofe_fun_equivI. *)
-  (*   epose proof (@ofe_fun_equivI _ (listVlC) (λ _, vlC -n> laterC (iProp Σ)) (λne ρ, λne v, CofeMor Next (Φ ρ v)) (λ ρ, λne v, Next (Ψ ρ v))). *)
-  (*   iDestruct (H0 with "Heq") as "?". *)
-
-  (*  "Heq" : (λ (ρ : listVlC) (v : vlC), Next (Φ ρ v)) *)
-  (*         ≡ (λ (ρ : listVlC) (v : vlC), Next (Ψ ρ v)) *)
-  (*   iDestruct (ofe_fun_equivI with "Heq"). as "?". *)
-  (*   by iDestruct (ofe_fun_equivI with "Heq") as "?". *)
-  (* Qed. *)
 End Sec.
