theories/lr_lemma.v
@@ -1,147 +1,60 @@
 Require Import Dot.tactics.
 Require Import Dot.unary_lr.
 
+Implicit Types T: ty.
+Implicit Types e: tm.
+
 Section Sec.
   Context `{HdotG: dotG Σ}.
 
-  Implicit Types T: ty.
-
-  (* XXX can we use instead |={⊤}=> ⟦T1⟧ ρ v -∗ ⟦T2⟧ ρ v? What I have below arose from iStpUvstp,
-     but a single modality seems more natural. However, using a single modality
-     is stronger, and for the current definition of WP and subtyping, *too* strong. *)
-  Definition uvstp1 Γ T1 T2: iProp Σ :=
-    (□∀ ρ v, ⟦Γ⟧*ρ -∗ (|={⊤}=> ⟦T1⟧ ρ v) ={⊤}=∗ ⟦T2⟧ ρ v)%I.
-  Global Arguments uvstp1 /.
-
-  Definition uvstp2 Γ T1 T2: iProp Σ :=
-    (□∀ ρ v, ⟦Γ⟧*ρ ={⊤}=∗ (⟦T1⟧ ρ v) → ⟦T2⟧ ρ v)%I.
-  Global Arguments uvstp2 /.
-  Print uvstp2.
-  Lemma uvstp21 Γ T1 T2: (uvstp2 Γ T1 T2 → uvstp1 Γ T1 T2)%I.
-  Proof.
-    iIntros "/= #Hstp !> * #Hg".
-    iDestruct ("Hstp" $! _ v with "Hg") as ">H".
-    iIntros ">HT1 !>". by iApply "H".
-  Qed.
-  Notation "Γ ⊨> T1 <: T2" := (uvstp1 Γ T1 T2) (at level 74, T1, T2 at next level).
-
-  (* False. *)
-  Lemma uvstp12 Γ T1 T2: (uvstp1 Γ T1 T2 -∗ uvstp2 Γ T1 T2)%I.
-  Proof.
-    iIntros "/= #Hstp !> * #Hg".
-    iSpecialize ("Hstp" $! ρ v with "Hg").
-    Fail iMod "Hstp".
-    Fail iApply "Hstp".
-    iIntros "!>".
-  Abort.
-
   Context (Γ: list ty).
-  (** If we can prove that vstp and stp are equivalent, we can use them interchangeably; and in my previous proofs, proving vstp was much easier. *)
-  Lemma iVstpStp T1 T2: (Γ ⊨ T1 <: T2 → Γ ⊨e T1 <: T2)%I.
-  Proof.
-    iIntros "/= #Hsub !> * #Hg HT1".
-    iApply (wp_wand with " [-]"). iApply "HT1". by iIntros; iApply "Hsub".
-  Qed.
 
-  (* Does the converse direction hold? Do we need it? *)
-  (* Lemma iStpVstp Γ T1 T2: (istp Γ T1 T2 -∗ ivstp Γ T1 T2)%I. *)
-  (* This direction is useful when we have istp as an hypothesis. *)
-  (* What I can easily prove: *)
-  Lemma iStpUvstp T1 T2: (Γ ⊨e T1 <: T2 -∗ Γ ⊨> T1 <: T2)%I.
-  Proof.
-    (* Inspired by the proof of wp_value_inv'! *)
-
-    (* More manual.*)
-    (* iIntros "/= #Hsub !> * #Hg *". *)
-    (* iSpecialize ("Hsub" $! (of_val v) with "Hg"). *)
-    (* rewrite !wp_unfold /wp_pre /=. by iApply "Hsub". *)
-    (* Restart. *)
-    iIntros "/= #Hsub !> * #Hg *".
-    setoid_rewrite wp_unfold.
-    by iApply ("Hsub" $! (of_val v)).
-  Qed.
-  Implicit Types e: tm.
-  (* To be able to use uvstp2, maybe we can use the following. Since it uses a single WP, it's clear
-   * that we're talking about a single execution of e! That's weaker for non-deterministic
-   * languages, but makes more sense: subtyping is about the same result after all.
-   *)
-  Definition istp2 Γ T1 T2 : iProp Σ := (□∀ e ρ, ⟦Γ⟧* ρ →
-                                                 WP e {{v, ⟦T1⟧ ρ v → ⟦T2⟧ ρ v}})%I.
-  Lemma iStpUvstp2 T1 T2: (istp2 Γ T1 T2 -∗ uvstp2 Γ T1 T2)%I.
-  Proof.
-    iIntros "/= #Hsub !> * #Hg *".
-    iSpecialize ("Hsub" $! (of_val v) with "Hg").
-    rewrite !wp_unfold /wp_pre /=. by iApply "Hsub".
-  Qed.
-
-  (* Maybe the update is OK; after all, it's part of the definition of weakest
-     preconditions, and it pairs with the later. But it confuses me honestly.
-
-     In any case, once we add pointers typing will clearly depend on resources (such as the heap), so we can just as well deal with it now. *)
-  (* Also, subtyping now implies subtyping after update: *)
-  Lemma vstpToUvstp T1 T2 : (Γ ⊨ T1 <: T2 → Γ ⊨> T1 <: T2)%I.
-    iIntros "#Hstp !> * #Hg > HT1 !>".
-    by iApply "Hstp".
-  Qed.
-  (* But not viceversa, because |==> P talks about the *existence* of a future resource world
-   where P holds, even though P might be false now. *)
-  Lemma uvstpToVstp T1 T2 : (Γ ⊨> T1 <: T2 → Γ ⊨ T1 <: T2)%I.
-    iIntros "/= #Hstp !> * #Hg #Ht1".
-    Fail iApply "Hstp".
-  Abort.
-
-  (* And subtyping later is enough to imply expression subtyping: *)
-  Lemma iVstpUpdatedStp T1 T2: (Γ ⊨> T1 <: T2 → Γ ⊨e T1 <: T2)%I.
-  Proof.
-    iIntros "/= #Hstp !> * #Hg HeT1".
-    by iApply (wp_strong_mono with "HeT1");
-      last (iIntros "* HT1"; iApply "Hstp").
-  Qed.
-
-  Lemma ivstp_later G T: G ⊨ T <: TLater T.
-  Proof. iIntros "!> ** /="; by iNext. Qed.
+  Lemma ivstp_later G T: G ⊨v T <: TLater T.
+  Proof. by iIntros "!> ** /=". Qed.
 
   (* So, value subtyping [ivstp] implies updated value subtyping [uvstp] but not
   viceversa. We can use the implication when proving value subtyping, but not
   when consuming its hypotheses. *)
   Lemma iuvstp_later T: Γ ⊨> T <: TLater T.
-  Proof. iApply vstpToUvstp. iIntros "!> ** /="; by iNext. Qed.
+  Proof. by iIntros "!> ** /=". Qed.
 
-  Lemma ivstp_ande1 T1 T2: Γ ⊨ TAnd T1 T2 <: T1.
+  Lemma ivstp_ande1 T1 T2: Γ ⊨> TAnd T1 T2 <: T1.
   Proof. by iIntros "/= !> * ? [? ?]". Qed.
-  Lemma ivstp_ande2 T1 T2: Γ ⊨ TAnd T1 T2 <: T2.
+  Lemma ivstp_ande2 T1 T2: Γ ⊨> TAnd T1 T2 <: T2.
   Proof. by iIntros "/= !> * ? [? ?]". Qed.
 
-  Lemma stp_andi T1 T2 ρ v:
-    ⟦T1⟧ ρ v -∗
-    ⟦T2⟧ ρ v -∗
-    ⟦TAnd T1 T2⟧ ρ v.
-  Proof. iIntros; by iSplit. Qed.
+  (* Lemma stp_andi T1 T2 ρ v: *)
+  (*   ⟦T1⟧ ρ v -∗ *)
+  (*   ⟦T2⟧ ρ v -∗ *)
+  (*   ⟦TAnd T1 T2⟧ ρ v. *)
+  (* Proof. iIntros; by iSplit. Qed. *)
 
   Lemma ivstp_andi S T1 T2:
-    Γ ⊨ S <: T1 -∗
-    Γ ⊨ S <: T2 -∗
-    Γ ⊨ S <: TAnd T1 T2.
+    Γ ⊨> S <: T1 -∗
+    Γ ⊨> S <: T2 -∗
+    Γ ⊨> S <: TAnd T1 T2.
   Proof.
     iIntros "/= #H1 #H2 !> * #Hg #HS".
-    iApply stp_andi; [iApply "H1" | iApply "H2"]; done.
+    iSpecialize ("H1" with "Hg"); iMod ("H1" with "HS") as "#H1'".
+    iSpecialize ("H2" with "Hg"); iMod ("H2" with "HS") as "#H2'".
+    naive_solver.
   Qed.
 
   Lemma stp_ori1 T1 T2 ρ v: ⟦T1⟧ ρ v -∗ ⟦TOr T1 T2⟧ ρ v.
-  Proof. iIntros "? /="; by iLeft. Qed.
+  Proof. iIntros "? /="; naive_solver. Qed.
   Lemma stp_ori2 T1 T2 ρ v: ⟦T2⟧ ρ v -∗ ⟦TOr T1 T2⟧ ρ v.
-  Proof. iIntros "? /="; by iRight. Qed.
+  Proof. iIntros "? /="; naive_solver. Qed.
 
   Lemma ivstp_ore S T1 T2:
-    Γ ⊨ T1 <: S -∗
-    Γ ⊨ T2 <: S -∗
-    Γ ⊨ TOr T1 T2 <: S.
+    Γ ⊨> T1 <: S -∗
+    Γ ⊨> T2 <: S -∗
+    Γ ⊨> TOr T1 T2 <: S.
   Proof. iIntros "/= #H1 #H2 !> * #Hg #[HT1 | HT2]"; [iApply "H1" | iApply "H2"]; done. Qed.
 
-  Lemma ivstp_ori1 T1 T2: Γ ⊨ T1 <: TOr T1 T2.
-  Proof. iIntros "!> ** /="; by iLeft. Qed.
-  Lemma ivstp_ori2 T1 T2: Γ ⊨ T2 <: TOr T1 T2.
-  Proof. iIntros "!> ** /="; by iRight. Qed.
+  Lemma ivstp_ori1 T1 T2: Γ ⊨> T1 <: TOr T1 T2.
+  Proof. iIntros "!> ** /="; naive_solver. Qed.
+  Lemma ivstp_ori2 T1 T2: Γ ⊨> T2 <: TOr T1 T2.
+  Proof. iIntros "!> ** /="; naive_solver. Qed.
 
   (*
      Γ, z: T₁ᶻ ⊨ T₁ᶻ <: T₂ᶻ
@@ -153,7 +66,7 @@ Section Sec.
     ivstp Γ (TMu T1) (TMu T2).
   Proof.
     iIntros "/= #Hstp !>" (v ρ) "#Hg #HT1".
-    iApply ("Hstp" $! v (v :: ρ)); by try iSplit.
+    iApply ("Hstp" $! v (v :: ρ)); naive_solver.
   Qed.
 
   (*
@@ -161,17 +74,18 @@ Section Sec.
      ----------------------------------------------- (<:-Bind-1)
      Γ ⊨ μ (x: T₁ˣ) <: T₂
   *)
+
   Lemma ivstp_mu_1 T1 T2:
-    ivstp (T1 :: Γ) T1 (T2.[up_ty_vl var_vl]) -∗
-    ivstp Γ (TMu T1) T2.
+    uvstp (T1 :: Γ) T1 (T2.[wkT]) -∗
+    uvstp Γ (TMu T1) T2.
   Proof.
-    iIntros "/= #Hstp !>" (v ρ) "#Hg #HT1".
+    iIntros "/= #Hstp !> * #Hg #HT1".
     (* Hopefully from a renaming/weakening lemma. *)
-    iAssert (interp T2 ρ v ≡ interp T2.[up_ty_vl var_vl] (v :: ρ) v)%I as "#Hren".
+    iAssert (interp T2 ρ v ≡ interp T2.[wkT] (v :: ρ) v)%I as "#Hren".
     { admit. }
     simpl.
     iRewrite "Hren".
-    iApply ("Hstp" $! v (v :: ρ)); by try iSplit.
+    iApply ("Hstp" $! v (v :: ρ)); naive_solver.
   Admitted.
 
   (*
@@ -180,12 +94,12 @@ Section Sec.
      Γ ⊨ T₁ <: μ(x: T₂ˣ)
   *)
   Lemma ivstp_mu_2 T1 T2:
-    ivstp (T1.[up_ty_vl var_vl] :: Γ) (T1.[up_ty_vl var_vl]) T2 -∗
-    ivstp Γ T1 (TMu T2).
+    uvstp (T1.[wkT] :: Γ) (T1.[wkT]) T2 -∗
+    uvstp Γ T1 (TMu T2).
   Proof.
     iIntros "/= #Hstp !>" (v ρ) "#Hg #HT1".
     (* Hopefully from a renaming/weakening lemma. *)
-    iAssert (interp T1 ρ v ≡ interp T1.[up_ty_vl var_vl] (v :: ρ) v)%I as "#Hren".
+    iAssert (interp T1 ρ v ≡ interp T1.[wkT] (v :: ρ) v)%I as "#Hren".
     { admit. }
     simpl.
     iRewrite "Hren" in "HT1".
