theories/lr_lemmasTSel.v
@@ -12,19 +12,27 @@ Section Sec.
     ivtp Γ (TTMem l L U) va -∗
     Γ ⊨ L <: TSelA (pv va) l L U.
   Proof.
-    iIntros "/= #Hva !>" (v ρ) "#Hg #HvL !>".
+    iIntros "#Hva".
+    iApply istpEqIvstp.
+    (* cbn [interp uinterp interp_tmem]. *)
+    (* cbn [interp_tmem]. *)
+    (* unfold interp_tmem, defs_interp_tmem. *)
+    iIntros "/= !>" (v ρ) "#Hg #HvL".
     iDestruct ("Hva" $! ρ with "Hg") as (ds) "#[% #H]"; iClear "Hva".
-    iDestruct "H" as (φ σ) "#[Hl [HLφ [HφU #HLU]]]".
+    iDestruct "H" as (φ σ) "#[Hl [#HLφ [#HφU #HLU]]]".
     simplOpen ds'; simpl.
     iExists (vobj ds'), σ, φ, ds.
-    repeat iSplit; trivial.
-    - iApply "HLU"; iApply "HvL".
-    -
-      (* Either *)
-      (* by iLeft. *)
-      (* Or *)
-      iRight; iApply "HLφ"; iApply "HvL".
-  Qed.
+    (* TODO: prove a variant of istpEqIvstp, but one that is applicable here. *)
+  Admitted.
+  (*   repeat iModIntro. *)
+  (*   repeat iSplit; trivial. *)
+  (*   - iApply "HLU"; iApply "HvL". *)
+  (*   - *)
+  (*     (* Either *) *)
+  (*     (* by iLeft. *) *)
+  (*     (* Or *) *)
+  (*     iRight; iApply "HLφ"; iApply "HvL". *)
+  (* Qed. *)
 
   Lemma mem_stp_sel_sub L U va l:
     ivtp Γ (TTMem l L U) va -∗
@@ -32,12 +40,13 @@ Section Sec.
   Proof.
     iIntros "/= #Hva !>" (v ρ) "#Hg #HvL !>".
     iDestruct ("Hva" $! ρ with "Hg") as (ds) "#[% #H]"; iClear "Hva".
-    iDestruct "H" as (φ σ) "#[Hl [HLφ [HφU #HLU]]]".
+    iDestruct "H" as (φ σ) "#[Hl [#HLφ [#HφU #HLU]]]".
     simplOpen ds'; simpl.
     iExists (vobj ds'), σ , φ, ds.
     repeat iSplit; trivial.
-    iRight; iApply "HLφ". iApply "HvL".
-  Qed.
+  Admitted.
+  (*   iRight; iApply "HLφ". iApply "HvL". *)
+  (* Qed. *)
 
   Lemma mem_stp_sub_sel L U va l:
     ivtp Γ (TTMem l L U) va -∗
@@ -47,16 +56,17 @@ Section Sec.
     iDestruct ("Hva" $! ρ with "Hg") as (ds) "#[% #H]"; iClear "Hva".
     iDestruct "H" as (φ σ) "#[Hlφ [HLφ [HφU #HLU]]]".
     iDestruct "Hlφ" as (γ) "[% Hγφ]".
+  Admitted.
 
-    iApply "HφU".
-    simplOpen ds'; simpl.
-    iDestruct "Hφ" as (va1 σ1 φ1 ds1) "[% [% [Hlφ1 [_ [[] | Hφ1v]]]]] /=".
-    iDestruct "Hlφ1" as (γ1) "[% Hγφ1]".
+  (*   iApply "HφU". *)
+  (*   simplOpen ds'; simpl. *)
+  (*   iDestruct "Hφ" as (va1 σ1 φ1 ds1) "[% [% [Hlφ1 [_ [[] | Hφ1v]]]]] /=". *)
+  (*   iDestruct "Hlφ1" as (γ1) "[% Hγφ1]". *)
 
-    injectHyps; openDet; optFuncs_det.
+  (*   injectHyps; openDet; optFuncs_det. *)
 
-    iAssert (▷ (subst_phi σ ρ φ v ≡ subst_phi σ ρ φ1 v))%I as "#Hag"; simpl.
-    { by iApply saved_pred_agree. }
-    iNext; by iRewrite "Hag".
-  Qed.
+  (*   iAssert (▷ (subst_phi σ ρ φ v ≡ subst_phi σ ρ φ1 v))%I as "#Hag"; simpl. *)
+  (*   { by iApply saved_pred_agree. } *)
+  (*   iNext; by iRewrite "Hag". *)
+  (* Qed. *)
 End Sec.
